WIP: implement SHA1

code/hash-new/Hacl.SHA1.fst
@@ -32,13 +32,51 @@ let init s =
   IB.recall_contents h0 (Seq.seq_of_list Spec.init_as_list);
   B.blit h0 0ul s 0ul 5ul
 
-let working_state_matches (h: HS.mem) (w: Spec.working_state) (s: state SHA1) : GTot Type0 =
-  let s' = B.as_seq h s in
-  w.Spec.a == Seq.index s' 0 /\
-  w.Spec.b == Seq.index s' 1 /\
-  w.Spec.c == Seq.index s' 2 /\
-  w.Spec.d == Seq.index s' 3 /\
-  w.Spec.e == Seq.index s' 4
+let working_state_of_seq (s: hash_w SHA1) : GTot Spec.working_state =
+  {
+    Spec.a = Seq.index s 0;
+    Spec.b = Seq.index s 1;
+    Spec.c = Seq.index s 2;
+    Spec.d = Seq.index s 3;
+    Spec.e = Seq.index s 4;
+  }
+
+let seq_of_working_state (s: Spec.working_state) : GTot (hash_w SHA1) =
+  (Seq.seq_of_list [
+    s.Spec.a;
+    s.Spec.b;
+    s.Spec.c;
+    s.Spec.d;
+    s.Spec.e;
+  ])
+
+let seq_of_working_state_of_seq (s: hash_w SHA1) : Lemma
+  (seq_of_working_state (working_state_of_seq s) `Seq.equal` s)
+  [SMTPat (seq_of_working_state (working_state_of_seq s))]
+= ()
+
+let working_state_of_seq_of_working_state (s: Spec.working_state) : Lemma
+  (working_state_of_seq (seq_of_working_state s) == s)
+  [SMTPat (working_state_of_seq (seq_of_working_state s))]
+= ()
+
+// NOTE: working_state_of_buffer MUST NOT be directly defined in terms
+// of working_state_of_seq. If it is, then step3_body below will not
+// typecheck
+
+let working_state_of_buffer (h: HS.mem) (s: state SHA1) : GTot Spec.working_state =
+  let s = B.as_seq h s in {
+    Spec.a = Seq.index s 0;
+    Spec.b = Seq.index s 1;
+    Spec.c = Seq.index s 2;
+    Spec.d = Seq.index s 3;
+    Spec.e = Seq.index s 4;
+  }
+
+let working_state_of_buffer_eq (h: HS.mem) (s: state SHA1) : Lemma
+  (working_state_of_buffer h s == working_state_of_seq (B.as_seq h s))
+  [SMTPat (working_state_of_buffer h s)]
+= ()
 
 inline_for_extraction
 let w_t = (b: B.lbuffer (word SHA1) 80)
@@ -46,16 +84,36 @@ let w_t = (b: B.lbuffer (word SHA1) 80)
 inline_for_extraction
 let block_t = (block: B.buffer U8.t { B.length block == size_block SHA1 } )
 
-let w_inv (h0: HS.mem) (h: HS.mem) (m: block_t) (b: w_t) (i: nat) : GTot Type0 =
+let w_inv' (i: nat) (mi: Spec.word_block) (b: w_t) (h: HS.mem) : GTot Type0 =
+  i <= 80 /\
+  B.live h b /\ (
+    let s = B.as_seq h b in
+    (forall (j: nat) .  {:pattern (Seq.index s j) } (j < i) ==> Spec.w mi (U32.uint_to_t j) == Seq.index s j)
+  )
+
+let w_inv = w_inv' 80
+
+let w_loop_inv (h0: Ghost.erased HS.mem) (m: block_t) (b: w_t) (h: HS.mem) (i: nat) : GTot Type0 =
+  let h0 = Ghost.reveal h0 in
+  i <= 80 /\
   B.disjoint m b /\
   B.live h0 m /\
   B.live h m /\
   B.live h b /\
   B.modifies (B.loc_buffer b) h0 h /\ (
-    let mi = E.seq_uint32_of_be size_block_w (B.as_seq h0 m) in
-    let s = B.as_seq h b in
-    (forall (j: nat) . (j < i /\ j < 80) ==> Spec.w mi (U32.uint_to_t j) == Seq.index s j)
+    let mi = E.seq_uint32_of_be size_block_w (B.as_seq h m) in
+    w_inv' i mi b h
   )
+
+let w_inv_elim (h: HS.mem) (m: Spec.word_block) (b: w_t) (i: nat) (j: nat) : Lemma
+  (requires (w_inv' i m b h /\ j < i))
+  (ensures (Seq.index (B.as_seq h b) j == Spec.w m (U32.uint_to_t j)))
+= ()
+
+let w_loop_inv_elim (h0: Ghost.erased HS.mem) (h: HS.mem) (m: block_t) (b: w_t) (i: nat) (j: nat) : Lemma
+  (requires (w_loop_inv h0 m b h i /\ j < i))
+  (ensures (Seq.index (B.as_seq h b) j == Spec.w (E.seq_uint32_of_be size_block_w (B.as_seq h m)) (U32.uint_to_t j)))
+= ()
 
 inline_for_extraction
 let index_32_be' (n: Ghost.erased nat) (b: B.buffer UInt8.t) (i: UInt32.t):
@@ -69,9 +127,9 @@ let index_32_be' (n: Ghost.erased nat) (b: B.buffer UInt8.t) (i: UInt32.t):
 = CE.index_32_be b i
 
 inline_for_extraction
-let w_body_value (h0: HS.mem) (m: block_t) (b: w_t) (i: U32.t) : HST.Stack U32.t
-  (requires (fun h -> w_inv h0 h m b (U32.v i) /\ U32.v i < 80))
-  (ensures (fun h v h' -> B.modifies B.loc_none h h' /\ v == Spec.w (E.seq_uint32_of_be size_block_w (B.as_seq h0 m)) i))
+let w_body_value (h0: Ghost.erased HS.mem) (m: block_t) (b: w_t) (i: U32.t) : HST.Stack U32.t
+  (requires (fun h -> w_loop_inv h0 m b h (U32.v i) /\ U32.v i < 80))
+  (ensures (fun h v h' -> B.modifies B.loc_none h h' /\ v == Spec.w (E.seq_uint32_of_be size_block_w (B.as_seq (Ghost.reveal h0) m)) i))
 = if U32.lt i 16ul
   then
     index_32_be' (Ghost.hide size_block_w) m i
@@ -82,16 +140,148 @@ let w_body_value (h0: HS.mem) (m: block_t) (b: w_t) (i: U32.t) : HST.Stack U32.t
     let wmit16 = B.index b (i `U32.sub` 16ul) in
     Spec.rotl 1ul (wmit3 `U32.logxor` wmit8 `U32.logxor` wmit14 `U32.logxor` wmit16)
 
+let lt_S_r (j i: nat) : Lemma
+  (requires (j < i + 1))
+  (ensures (j = i \/ j < i))
+= ()
+
+inline_for_extraction
+let w_body (h0: Ghost.erased HS.mem) (m: block_t) (b: w_t) (i: U32.t { U32.v i < 80 }) : HST.Stack unit
+  (requires (fun h -> w_loop_inv h0 m b h (U32.v i)))
+  (ensures (fun _ _ h' -> w_loop_inv h0 m b h' (U32.v i + 1)))
+= let h = HST.get () in
+  let v = w_body_value h0 m b i in
+  B.upd b i v;
+  let h' = HST.get () in
+  let f (j: nat) : Lemma
+    (requires (j < U32.v i + 1))
+    (ensures (j < U32.v i + 1 /\ Seq.index (B.as_seq h' b) j == Spec.w (E.seq_uint32_of_be size_block_w (B.as_seq (Ghost.reveal h0) m)) (U32.uint_to_t j)))
+  = lt_S_r j (U32.v i);
+    if j = U32.v i
+    then ()
+    else w_loop_inv_elim h0 h m b (U32.v i) j
+  in
+  Classical.forall_intro (Classical.move_requires f)
+
+inline_for_extraction
+let w (m: block_t) (b: w_t) : HST.Stack unit
+  (requires (fun h -> B.live h m /\ B.live h b /\ B.disjoint m b))
+  (ensures (fun h _ h' -> B.modifies (B.loc_buffer b) h h' /\ w_inv (E.seq_uint32_of_be size_block_w (B.as_seq h m)) b h'))
+= let h = Ghost.hide (HST.get ()) in
+  C.Loops.for 0ul 80ul (w_loop_inv h m b) (fun i -> w_body h m b i)
+
+inline_for_extraction
+let step3_body
+  (mi: Ghost.erased Spec.word_block)
+  (w: w_t)
+  (b: state SHA1)
+  (t: U32.t {U32.v t < 80})
+: HST.Stack unit
+  (requires (fun h ->
+    w_inv (Ghost.reveal mi) w h /\
+    B.live h b /\
+    B.disjoint w b
+  ))
+  (ensures (fun h _ h' ->
+    B.modifies (B.loc_buffer b) h h' /\
+    working_state_of_buffer h' b == Spec.step3_body' (Ghost.reveal mi) (working_state_of_buffer h b) t
+  ))
+= let _a = B.index b 0ul in
+  let _b = B.index b 1ul in
+  let _c = B.index b 2ul in
+  let _d = B.index b 3ul in
+  let _e = B.index b 4ul in
+  let wmit = B.index w t in
+  let _T = Spec.rotl 5ul _a `U32.add_mod` Spec.f t _b _c _d `U32.add_mod` _e `U32.add_mod` Spec.k t `U32.add_mod` wmit in
+  B.upd b 4ul _d;
+  B.upd b 3ul _c;
+  B.upd b 2ul (Spec.rotl 30ul _b);
+  B.upd b 1ul _a;
+  B.upd b 0ul _T
+
+inline_for_extraction
+let zero_out
+  (b: B.buffer U32.t)
+  (len: U32.t { U32.v len == B.length b })
+: HST.Stack unit
+  (requires (fun h -> B.live h b))
+  (ensures (fun h _ h' -> B.modifies (B.loc_buffer b) h h' /\ B.live h' b))
+= let h0 = HST.get () in
+  C.Loops.for 0ul len (fun h _ -> B.live h b /\ B.modifies (B.loc_buffer b) h0 h) (fun i -> B.upd b i 0ul)
+
+let spec_step3_body (mi: Spec.word_block) (st: Ghost.erased (hash_w SHA1)) (t: nat {t < 80}) : Tot (Ghost.erased (hash_w SHA1)) =
+  Ghost.elift1 (fun h -> seq_of_working_state (Spec.step3_body mi (working_state_of_seq h) t)) st
+
+let spec_step3_body_spec (mi: Spec.word_block) (st: Ghost.erased (hash_w SHA1)) (t: nat { t < 80 } ) : Lemma
+  (working_state_of_seq (Ghost.reveal (spec_step3_body mi st t)) == Spec.step3_body mi (working_state_of_seq (Ghost.reveal st)) t)
+  [SMTPat (working_state_of_seq (Ghost.reveal (spec_step3_body mi st t)))]
+= ()
+
+let repeat_range_spec_step3_body (mi: Spec.word_block) (st: Ghost.erased (hash_w SHA1)) (i j: nat) : Lemma
+  (requires (i <= j /\ j < 80))
+  (ensures (working_state_of_seq (Ghost.reveal (Spec.Loops.repeat_range i j (spec_step3_body mi) st)) ==
+  Spec.Loops.repeat_range i j (Spec.step3_body mi) (working_state_of_seq (Ghost.reveal st))
+  ))
+= admit ()
+
+inline_for_extraction
+let impl_step3_body
+  (mi: Ghost.erased Spec.word_block)
+  (w: w_t)
+  (b: state SHA1)
+  (t: U32.t {U32.v t < 80})
+: HST.Stack unit
+  (requires (fun h ->
+    w_inv (Ghost.reveal mi) w h /\
+    B.live h b /\
+    B.disjoint w b
+  ))
+  (ensures (fun h _ h' ->
+    B.modifies (B.loc_buffer b) h h' /\
+    B.as_seq h' b == Ghost.reveal (spec_step3_body (Ghost.reveal mi) (Ghost.hide (B.as_seq h b)) (U32.v t))
+  ))
+= step3_body mi w b t
+
+#set-options "--z3rlimit 16"
+
 (*
-let w_body (h0: HS.mem) (m: block_t) (b: w_t) (i: U32.t) : HST.Stack unit
-  (requires (fun h -> w_inv h0 h m b (U32.v i) /\ U32.v i < 80))
-  (ensures (fun _ _ h' -> w_inv h0 h' m b (U32.v i + 1)))
-= if U32.lt i 16ul
-  then B.upd b i (CE.index_32_be m i)
-  else
-    let wmit3 = B.index b (i `U32.sub` 3ul) in
-    let wmit8 = B.index b (i `U32.sub` 8ul) in
-    let wmit14 = B.index b (i `U32.sub` 14ul) in
-    let wmit16 = B.index b (i `U32.sub` 16ul) in
-    let v = Spec.rotl 1ul (wmit3 `U32.logxor` wmit8 `U32.logxor` wmit14 `U32.logxor` wmit16) in
-    B.upd b i v
+inline_for_extraction
+let step3
+  (m: block_t)
+  (h: state SHA1)
+: HST.Stack unit
+  (requires (fun h0 ->
+    B.live h0 m /\
+    B.live h0 h /\
+    B.disjoint m h
+  ))
+  (ensures (fun h0 _ h1 ->
+    B.modifies (B.loc_buffer h) h0 h1 /\
+    B.live h1 h /\
+    working_state_of_buffer h1 h == Spec.step3 (E.seq_uint32_of_be size_block_w (B.as_seq h0 m)) (B.as_seq h0 h)
+  ))
+= let h0 = HST.get () in
+  HST.push_frame ();
+  let _w = B.alloca 0ul 80ul in
+  w m _w;
+  let mi = Ghost.hide (E.seq_uint32_of_be size_block_w (B.as_seq h0 m)) in
+  let h1 = HST.get () in
+  let inv (h' : HS.mem) : GTot Type0 =
+    B.modifies (B.loc_buffer h) h1 h'
+  in
+  let fc (i: U32.t { U32.v i < 80 } ) : HST.Stack unit
+    (requires (fun h2 -> inv h2 /\ B.live h2 h))
+    (ensures (fun h2 _ h3 -> B.live h2 h /\ B.live h3 h /\ B.modifies (B.loc_buffer h) h2 h3 /\ inv h3 /\ B.as_seq h3 h == Ghost.reveal (spec_step3_body (Ghost.reveal mi) (Ghost.hide (B.as_seq h2 h)) (U32.v i))
+    ))
+  = admit ()
+  in
+  let _ = C.Loops.repeat_range 5ul 0ul 80ul (spec_step3_body (Ghost.reveal mi)) h inv  fc in
+  admit ();
+  repeat_range_spec_step3_body (Ghost.reveal mi) (Ghost.hide (B.as_seq h1 h)) 0 80;
+  zero_out _w 80ul;
+  HST.pop_frame ();
+  ()
+
+
+(*
+(fun i -> impl_step3_body mi _w h i)
